theories/iris_fundamental_block.v
@@ -21,39 +21,26 @@ Section fundamental.
   (* -------------------------------------- EXPRESSIONS ------------------------------------ *)
   (* --------------------------------------------------------------------------------------- *)
 
-  (* ----------------------------------------- LOOP ---------------------------------------- *)
-
-  Lemma interp_ctx_continuations_push_label_loop lh C i tm tn es :
+  Lemma interp_ctx_continuations_push_label_block lh C i tm :
     base_is_empty lh ->
     lholed_lengths (rev (tc_label C)) lh ->
-    □ (∀ (a : leibnizO frame) (a0 : seq.seq (leibnizO value)),
-           ⌜length a0 = length tn⌝
-           →  ↪[frame]a -∗
-               interp_frame (tc_local C) i a -∗
-             □ ([∗ list] w;τ ∈ a0;tn, interp_value τ w) -∗
-             WP of_val (immV a0) ++ to_e_list [BI_loop (Tf tn tm) es]
-             {{ vs,
-                (interp_val tm vs
-                 ∨ interp_br (tc_local C) i vs lh (tc_label C)) ∗
-                (∃ f0 : leibnizO frame,  ↪[frame]f0 ∗
-                   interp_frame (tc_local C) i f0) }}) -∗
-      interp_ctx_continuations (tc_label C) (tc_local C) i lh -∗
-      interp_ctx_continuation (tc_label (upd_label C ([tn] ++ tc_label C))) (push_base lh (length tn) [AI_basic (BI_loop (Tf tn tm) es)] [] [])
-                              0 tn (tc_local C) i.
+    interp_ctx_continuations (tc_label C) (tc_local C) i lh -∗
+    interp_ctx_continuation (tc_label (upd_label C ([tm] ++ tc_label C))) (push_base lh (length tm) [] [] [])
+                              0 tm (tc_local C) i.
   Proof.
-    iIntros (Hlh_base Hlh_len) "#HIH #Hc". unfold interp_ctx_continuation.
+    iIntros (Hlh_base Hlh_len) "#Hc". unfold interp_ctx_continuation.
     iSimpl. rewrite lh_depth_push_base.
     assert (S (lh_depth lh) - 1 = lh_depth lh) as ->;[lia|].
     rewrite get_layer_push_base_0;[|auto].
-    apply lh_minus_push_base_Some with (n:=length tn) (es:=[AI_basic (BI_loop (Tf tn tm) es)]) (vs1:=[]) (es2:=[]) in Hlh_base as Hmin.
-    iExists _,_,_,_,_,_. repeat (iSplit;[eauto|]).
+    apply lh_minus_push_base_Some with (n:=length tm) (es:=[]) (vs1:=[]) (es2:=[]) in Hlh_base as Hmin.
+    iExists _,_,_,_,_,_. repeat (iSplit;[simpl;eauto|]).
     iModIntro. iIntros (v f).
     iIntros "#Hw [Hf Hfv]".
     unfold interp_expression.
     rewrite app_nil_l app_nil_r.
 
     iDestruct "Hw" as "[-> | Hv]".
-    { iClear "HIH". iExists [].
+    { iExists [].
       take_drop_app_rewrite_twice 0 1.
       iApply (wp_wand _ _ _ (λ vs, ⌜vs = trapV⌝ ∗  ↪[frame]f)%I with "[Hf]").
       { iApply (wp_trap with "[] [Hf]");auto. }
@@ -62,34 +49,26 @@ Section fundamental.
     iDestruct "Hv" as (ws' ->) "Hv". iExists tm.
     iDestruct (big_sepL2_length with "Hv") as %Hlen.
     repeat rewrite -!/(interp_frame _ _ _).
-    iApply ("HIH" with "[] Hf Hfv Hv");eauto. 
+    rewrite app_nil_r.
+    iApply wp_value;[done|].
+    iSplitR;[|iExists _;iFrame;iExists _;eauto].
+    iLeft. iRight. iExists _. eauto.
   Qed.
 
-  Lemma interp_ctx_push_label_loop C tm i lh tn es :
-    □ (∀ (a : leibnizO frame) (a0 : seq.seq (leibnizO value)),
-           ⌜length a0 = length tn⌝
-           →  ↪[frame]a -∗
-               interp_frame (tc_local C) i a -∗
-             □ ([∗ list] w;τ ∈ a0;tn, interp_value τ w) -∗
-             WP of_val (immV a0) ++ to_e_list [BI_loop (Tf tn tm) es]
-             {{ vs,
-                (interp_val tm vs
-                 ∨ interp_br (tc_local C) i vs lh (tc_label C)) ∗
-                (∃ f0 : leibnizO frame,  ↪[frame]f0 ∗
-                   interp_frame (tc_local C) i f0) }}) -∗
+  Lemma interp_ctx_push_label_block C tm i lh :
     interp_ctx (tc_label C) (tc_local C) i lh -∗
-    interp_ctx (tc_label (upd_label C ([tn] ++ tc_label C)%list))
-      (tc_local (upd_label C ([tn] ++ tc_label C)%list)) i
-      (push_base lh (length tn) [AI_basic (BI_loop (Tf tn tm) es)] [] []).
+    interp_ctx (tc_label (upd_label C ([tm] ++ tc_label C)%list))
+      (tc_local (upd_label C ([tm] ++ tc_label C)%list)) i
+      (push_base lh (length tm) [] [] []).
   Proof.
-    iIntros "#HIH [%Hlh_base [%Hlh_len [%Hlh_valid #Hc]]]".
+    iIntros "[%Hlh_base [%Hlh_len [%Hlh_valid #Hc]]]".
     iSplit;[|iSplit;[|iSplit]].
     { iPureIntro. apply base_is_empty_push_base. }
     { iPureIntro. apply lholed_lengths_push_base. auto. }
     { iPureIntro. apply lholed_valid_push_base. auto. }
     { iSplitR.
       { iSimpl. iSplitR;[|done].
-        iApply (interp_ctx_continuations_push_label_loop with "[] []");auto. }
+        iApply (interp_ctx_continuations_push_label_block with "[]");auto. }
       iApply (big_sepL_mono with "Hc").
       iIntros (k y Hk). iSimpl.
       iIntros "#Hcont".
@@ -106,34 +85,23 @@ Section fundamental.
     }
   Qed.
 
-  Lemma interp_br_step C (j : nat) (vh: valid_holed j) m vs tn p i es tm lh f' :
-    m = length tn ->
+  Lemma interp_br_step C (j : nat) (vh: valid_holed j) m vs p i tm lh f' :
+    m = length tm ->
     get_base_l vh = vs ->
     lh_depth (lh_of_vh vh) = p ->
     j = p ->
-    □ (∀ a a0, ⌜length a0 = length tn⌝ →
-               ↪[frame]a -∗ interp_frame (tc_local C) i a -∗
-             □ ([∗ list] w;τ ∈ a0;tn, interp_value τ w) -∗
-             WP ((λ v : value, AI_basic (BI_const v)) <$> a0) ++
-                to_e_list [BI_loop (Tf tn tm) es]
-             {{ vs0,
-                (interp_val tm vs0
-                 ∨ interp_br (tc_local C) i vs0 lh (tc_label C)) ∗
-                (∃ f0 : leibnizO frame,  ↪[frame]f0 ∗
-                                          interp_frame (tc_local C) i f0) }}) -∗
-      interp_br_body (tc_label (upd_label C ([tn] ++ tc_label C)))
-                     (push_base lh (length tn) [AI_basic (BI_loop (Tf tn tm) es)] [] [])
-                     j p vs (tc_local C) i -∗
-      ↪[frame]f' -∗
-      interp_frame (tc_local C) i f' -∗
-      WP [AI_label m [AI_basic (BI_loop (Tf tn tm) es)]
-        (vfill vh [AI_basic (BI_br j)])]
+    interp_br_body (tc_label (upd_label C ([tm] ++ tc_label C)))
+                   (push_base lh (length tm) [] [] [])
+                   j p vs (tc_local C) i -∗
+    ↪[frame]f' -∗
+    interp_frame (tc_local C) i f' -∗
+    WP [AI_label m [] (vfill vh [AI_basic (BI_br j)])]
       {{ v, (interp_val tm v ∨ interp_br (tc_local C) i v lh (tc_label C)) ∗
            (∃ f0,  ↪[frame]f0 ∗ interp_frame (tc_local C) i f0) }}.
   Proof.
-    iIntros (Hlen Hbase Hsize e) "#IH Hbr Hf Hfv".
+    iIntros (Hlen Hbase Hsize e) "Hbr Hf Hfv".
     unfold interp_br_body.
-    destruct (pull_base_l_drop_len vh (length vs - length tn)) eqn:Hpb.
+    destruct (pull_base_l_drop_len vh (length vs - length tm)) eqn:Hpb.
     erewrite vfill_pull_base_l_take_len;[|eauto].
     pose proof (vfill_to_lfilled v (((λ x : value, AI_basic (BI_const x)) <$> l) ++ [AI_basic (BI_br j)])) as [k [Hle Hfill]].
     apply lfilled_depth in Hfill as Hdepth.
@@ -152,52 +120,32 @@ Section fundamental.
     { apply const_list_of_val. }
     { rewrite fmap_length. eapply length_pull_base_l_take_len in Hpb;[|eauto]. rewrite Hpb.
       rewrite Hlen.
-      assert (length vs >= length tn);[|lia]. rewrite Hlen2. lia. }
+      assert (length vs >= length tm);[|lia]. rewrite Hlen2. lia. }
     iNext. iIntros "Hf".
-    iApply ("IH" with "[] Hf Hfv");auto.
-    { iPureIntro. erewrite length_pull_base_l_take_len;eauto.
-      assert (length vs >= length tn);[|lia]. rewrite Hlen2. lia. }
-    { eapply take_drop_pull_base_l_take_len in Hpb as Happ;[|eauto..];[|lia].
-      rewrite Happ.
-      iDestruct (big_sepL2_app_inv with "Hvalvs") as "[? ?]".
-      { right. eapply length_pull_base_l_take_len in Hpb;[|eauto]. rewrite Hpb.
-        assert (length vs >= length tn);[|lia]. rewrite Hlen2. lia. }
-      iModIntro. iFrame "#".
-    }
+    rewrite app_nil_r.
+    rewrite of_val_imm.
+    iApply wp_value;[done|].
+    iSplitR "Hfv Hf";[|iExists _;iFrame;iExists _;eauto].
+    iLeft. iRight. iExists _. iSplit;eauto.
+    eapply take_drop_pull_base_l_take_len in Hpb as Happ;[|eauto..];[|lia].
+    rewrite Happ.
+    iDestruct (big_sepL2_app_inv with "Hvalvs") as "[? ?]".
+    { right. eapply length_pull_base_l_take_len in Hpb;[|eauto]. rewrite Hpb.
+      assert (length vs >= length tm);[|lia]. rewrite Hlen2. lia. }
+    iFrame "#".
   Qed.
 
-  Lemma interp_br_stuck C (j : nat) (vh: valid_holed j) m vs tn p i es tm lh f' :
-    m = length tn ->
-    get_base_l vh = vs ->
-    lh_depth (lh_of_vh vh) = p ->
-    j ≠ p ->
-    lholed_lengths (rev (tc_label C)) lh ->
-    lholed_valid lh ->
-    base_is_empty lh ->
-    interp_br_body (tc_label (upd_label C ([tn] ++ tc_label C)))
-                   (push_base lh (length tn) [AI_basic (BI_loop (Tf tn tm) es)] [] [])
-                   j p vs (tc_local C) i -∗
-    ↪[frame]f' -∗
-    interp_frame (tc_local C) i f' -∗
-    WP [AI_label m [AI_basic (BI_loop (Tf tn tm) es)]
-        (vfill vh [AI_basic (BI_br j)])]
-      {{ v, (interp_val tm v ∨ interp_br (tc_local C) i v lh (tc_label C)) ∗
-           (∃ f0,  ↪[frame]f0 ∗ interp_frame (tc_local C) i f0) }}.
-  Proof.
-    iIntros (Hlen Hbase Hsize n Hlh_length Hlh_valid Hlh_empty) "Hbr Hf Hfv".
-    iApply (interp_br_stuck_push with "Hbr Hf Hfv");eauto.
-  Qed.
+  (* ----------------------------------------- BLOCK --------------------------------------- *)
 
-  Lemma typing_loop C es tn tm : (⊢ semantic_typing (HWP:=HWP) (upd_label C ([tn] ++ tc_label C)%list) (to_e_list es) (Tf tn tm)) ->
-                                 ⊢ semantic_typing (HWP:=HWP) C (to_e_list [BI_loop (Tf tn tm) es]) (Tf tn tm).
+  Lemma typing_block C tn tm es : (⊢ semantic_typing (HWP:=HWP) (upd_label C ([tm] ++ tc_label C)%list) (to_e_list es) (Tf tn tm)) ->
+                                  ⊢ semantic_typing (HWP:=HWP) C (to_e_list [BI_block (Tf tn tm) es]) (Tf tn tm).
   Proof.
     intros IHbe_typing.
     unfold semantic_typing, interp_expression.
     iIntros (i lh).
     iIntros "#Hi".
     
-    iDestruct (IHbe_typing $! i (push_base lh (length tn) [AI_basic (BI_loop (Tf tn tm) es)]
-                                           [] []) with "[]") as "HH"; [by (destruct C,i;eauto)|].
+    iDestruct (IHbe_typing $! i (push_base lh (length tm) [] [] []) with "[]") as "HH"; [by (destruct C,i;eauto)|].
 
     iIntros "#Hc". iIntros (f vs) "[Hf Hfv] #Hv".
     
@@ -209,10 +157,7 @@ Section fundamental.
     iDestruct "Hv" as (ws ->) "Hv".
     iDestruct (big_sepL2_length with "Hv") as %Hlen.
 
-    iRevert "Hfv Hv". iLöb as "IH"
-  forall (f ws Hlen).
-    iIntros "Hlocs #Hv".
-    iApply (wp_loop with "Hf");eauto.
+    iApply (wp_block with "Hf");eauto.
     { apply v_to_e_is_const_list. }
     { rewrite fmap_length //. }
     iNext. iIntros "Hf".
@@ -226,7 +171,7 @@ Section fundamental.
                       ∗ ∃ f, ↪[frame] f ∗ interp_frame (tc_local C) i f }})%I as "Hcont".
     { iIntros (f') "Hfv Hf".
       iDestruct ("HH" with "[] [Hf Hfv] []") as "Hcont".
-      { iApply (interp_ctx_push_label_loop with "[$] [$]"). }
+      { iApply (interp_ctx_push_label_block with "[$]"). }
       { iFrame "∗ #". }
       { iRight. iExists _. eauto. }
       iApply (wp_wand with "Hcont").
@@ -246,7 +191,7 @@ Section fundamental.
     iDestruct "Hred" as "[#Hval | Hbr]".
     
     { iDestruct "Hval" as (vs ->) "Hval".
-      rewrite fmap_length Hlen. iDestruct (big_sepL2_length with "Hval") as %Hlen'.
+      iDestruct (big_sepL2_length with "Hval") as %Hlen'.
       iApply (wp_wand_ctx _ _ _ (λ vs, ⌜vs = immV _⌝ ∗ _)%I with "[Hf]").
       { iApply (wp_val_return with "Hf");[apply const_list_of_val|].
         iIntros "Hf". rewrite app_nil_l app_nil_r.
@@ -258,19 +203,18 @@ Section fundamental.
     { rewrite fixpoint_interp_br_eq.
       iDestruct "Hbr" as (j vh vs p -> Hbase Hsize) "Hbr".
       simpl of_val.
-
-      rewrite fmap_length.
-      assert (LH_rec [] (length ws) [AI_basic (BI_loop (Tf tn tm) es)] (LH_base [] []) [] =
-                push_base (LH_base [] []) (length ws) [AI_basic (BI_loop (Tf tn tm) es)] [] []) as Heq;[auto|].
+      
+      assert (LH_rec [] (length tm) [] (LH_base [] []) [] =
+                push_base (LH_base [] []) (length tm) [] [] []) as Heq;[auto|].
       rewrite Heq.
       iApply wp_label_push_nil_inv. iApply wp_wasm_empty_ctx.
 
       destruct (decide (j = p)).
-      { iApply (interp_br_step with "[] Hbr Hf Hfv");eauto. }
+      { iApply (interp_br_step with "Hbr Hf Hfv");eauto. }
 
       { iAssert (⌜lholed_lengths (rev (tc_label C)) lh⌝ ∧ ⌜lholed_valid lh⌝ ∧ ⌜base_is_empty lh⌝)%I as %[Hlh_length [Hlh_valid Hlh_empty]].
         { iDestruct "Hc" as "[% [% [% _]]]". auto. }
-        iApply (interp_br_stuck with "Hbr Hf Hfv");eauto. }
+        iApply (interp_br_stuck_push with "Hbr Hf Hfv");eauto. }
     }
   Qed.
 
