theories/iris_fundamental_if.v
@@ -1,0 +1,83 @@
+From mathcomp Require Import ssreflect eqtype seq ssrbool.
+From iris.program_logic Require Import language.
+From iris.proofmode Require Import base tactics classes.
+From iris.base_logic Require Export gen_heap ghost_map proph_map na_invariants.
+From iris.base_logic.lib Require Export fancy_updates.
+From iris.algebra Require Import list.
+From iris.prelude Require Import options.
+
+Require Export iris iris_locations iris_properties iris_atomicity stdpp_aux.
+Require Export iris_rules.
+Require Export datatypes host operations properties opsem typing.
+Require Export iris_logrel iris_fundamental_helpers iris_fundamental_block.
+Import uPred.
+
+Section fundamental.
+  Import DummyHosts. (* placeholder *)
+
+  Context `{!wfuncG Σ, !wtabG Σ, !wtabsizeG Σ, !wmemG Σ, !wmemsizeG Σ, !wglobG Σ, !wframeG Σ, HWP: host_program_logic, !logrel_na_invs Σ}.
+  
+  (* --------------------------------------------------------------------------------------- *)
+  (* -------------------------------------- EXPRESSIONS ------------------------------------ *)
+  (* --------------------------------------------------------------------------------------- *)
+
+  (* ----------------------------------------- IF ------------------------------------------ *)
+
+  Lemma typing_if C tn tm es1 es2 : (⊢ semantic_typing (HWP:=HWP) (upd_label C ([tm] ++ tc_label C)%list) (to_e_list es1) (Tf tn tm)) ->
+                                    (⊢ semantic_typing (HWP:=HWP) (upd_label C ([tm] ++ tc_label C)%list) (to_e_list es2) (Tf tn tm)) ->
+                                    ⊢ semantic_typing (HWP:=HWP) C (to_e_list [BI_if (Tf tn tm) es1 es2]) (Tf (tn ++ [T_i32]) tm).
+  Proof.
+    intros IHbe_typing1 IHbe_typing2.
+    unfold semantic_typing, interp_expression.
+    iIntros (i lh).
+    iIntros "#Hi #Hc". iIntros (f vs) "[Hf Hfv] #Hv".
+    
+    iDestruct "Hv" as "[-> | Hv]".
+    {  take_drop_app_rewrite_twice 0 1.
+       iApply (wp_wand _ _ _ (λ vs, ⌜vs = trapV⌝ ∗  ↪[frame]f)%I with "[Hf]").
+       { iApply (wp_trap with "[] [Hf]");auto. }
+       iIntros (v0) "[? ?]". iFrame. iExists _. iFrame "∗ #". }
+    iDestruct "Hv" as (ws ->) "Hv".
+    iDestruct (big_sepL2_length with "Hv") as %Hlen.
+    assert (exists w ws', ws = ws' ++ [w]) as [w [ws' ->]].
+    { induction ws using rev_ind;eauto. destruct tn =>//. }
+    iDestruct (big_sepL2_app_inv with "Hv") as "[Hws' Hw]";[by right|].
+    simpl of_val. rewrite fmap_app. rewrite -app_assoc.
+    iApply iRewrite_nil_r. rewrite -app_assoc.
+    iApply wp_wasm_empty_ctx.
+    iApply wp_base_push.
+    { apply const_list_of_val. }
+    iSimpl.
+    iSimpl in "Hw". iDestruct "Hw" as "[Hw _]".
+    iDestruct "Hw" as (n) "->".
+    
+    destruct (Wasm_int.Int32.eq_eqP n (Wasm_int.int_zero i32m)).
+
+    { iApply (wp_if_false_ctx with "Hf");[auto|].
+      iNext. iIntros "Hf".
+
+      apply typing_block in IHbe_typing2.
+      iDestruct (IHbe_typing2 $! i lh with "[]") as "HH2"; [by (destruct C,i;eauto)|].
+      iIntros (LI HLI%lfilled_Ind_Equivalent).
+      inversion HLI;simplify_eq. erewrite app_nil_r.
+      rewrite -/(of_val (immV ws')).
+      unfold interp_expression. simpl to_e_list.
+      iApply ("HH2" with "[] [Hf Hfv]");iFrame "∗ #".
+      iRight. iExists _. iSplit;eauto.
+    }
+    { iApply (wp_if_true_ctx with "Hf");[auto|].
+      iNext. iIntros "Hf".
+
+      apply typing_block in IHbe_typing1.
+      iDestruct (IHbe_typing1 $! i lh with "[]") as "HH2"; [by (destruct C,i;eauto)|].
+      iIntros (LI HLI%lfilled_Ind_Equivalent).
+      inversion HLI;simplify_eq. erewrite app_nil_r.
+      rewrite -/(of_val (immV ws')).
+      unfold interp_expression. simpl to_e_list.
+      iApply ("HH2" with "[] [Hf Hfv]");iFrame "∗ #".
+      iRight. iExists _. iSplit;eauto.
+    }
+  Qed.
+    
+
+End fundamental.
